Update our horizontal composition prototype

common/ModuleSemantics.v
@@ -7,91 +7,43 @@ Require Import Globalenvs.
 Require Import Integers.
 Require Import Smallstep.
 
-Module Res.
-  Section RESOLVE.
-    Context (L: Smallstep.semantics).
-    Context (internal: query -> bool).
-
-    Definition cont: Type := reply -> state L -> Prop.
-
-    Definition external_event (t: trace) :=
-      match t with
-        | Event_extcall _ _ q r :: nil => internal q = false
-        | _ => True
-      end.
-
-    Definition current_continuation (s: Smallstep.state L) f sg q: cont :=
-      fun r s' =>
-        Smallstep.step L (globalenv L) s (Event_extcall f sg q r :: nil) s'.
-
-    Inductive state := State (s: Smallstep.state L) (k: list cont).
-
-    Inductive initial_state (q: query): state -> Prop :=
-      | initial_state_intro s:
-          Smallstep.initial_state L q s ->
-          initial_state q (State s nil).
-
-    Inductive final_state: state -> reply -> Prop :=
-      | final_state_intro s r:
-          Smallstep.final_state L s r ->
-          final_state (State s nil) r.
-
-    Inductive step ge : state -> trace -> state -> Prop :=
-      | step_internal s t s' stk:
-          Smallstep.step L ge s t s' ->
-          external_event t ->
-          step ge (State s stk) t (State s' stk)
-      | step_call s stk f sg q si:
-          let k := current_continuation s f sg q in
-          (exists r s', k r s') ->
-          Smallstep.initial_state L q si ->
-          step ge (State s stk) E0 (State si (k::stk))
-      | step_return si (k: cont) stk r s:
-          Smallstep.final_state L si r ->
-          k r s ->
-          step ge (State si (k::stk)) E0 (State s stk).
-
-    Definition semantics: Smallstep.semantics :=
-      {|
-        Smallstep.state := state;
-        Smallstep.step := step;
-        Smallstep.initial_state := initial_state;
-        Smallstep.final_state := final_state;
-        Smallstep.globalenv := globalenv L;
-        Smallstep.symbolenv := symbolenv L;
-      |}.
-
-    Lemma step_external_event ge s t s':
-      step ge s t s' ->
-      external_event t.
-    Proof.
-      destruct 1; simpl; eauto.
-    Qed.
-  End RESOLVE.
-End Res.
-
 (** * Flat composition *)
+
+(** The flat composition of transition systems essentially corresponds
+  to the union of strategies: if component [i] handles a given query,
+  then the flat composition will handle it in a similar way. However,
+  the components cannot call each other. *)
 
 Module FComp.
   Section FLATCOMP.
     Context (ge: Senv.t).
-    Context {I} (L: I -> semantics).
+    Context {li1 li2 I} (L: I -> semantics li1 li2).
 
     Definition genv := forall i, genvtype (L i).
 
     Definition state := { i : I & state (L i) }.
 
     Inductive step (ge: genv): state -> trace -> state -> Prop :=
-      step_intro i s t s':
-        Smallstep.step (L i) (ge i) s t s' ->
-        step ge (existT _ i s) t (existT _ i s').
+      | step_intro i s t s':
+          Smallstep.step (L i) (ge i) s t s' ->
+          step ge (existT _ i s) t (existT _ i s').
 
-    Inductive initial_state (q: query): state -> Prop :=
-      initial_state_intro i s:
-        Smallstep.initial_state (L i) q s ->
-        initial_state q (existT _ i s).
+    Inductive initial_state (q: query li2): state -> Prop :=
+      | initial_state_intro i s:
+          Smallstep.initial_state (L i) q s ->
+          initial_state q (existT _ i s).
 
-    Definition final_state (s: state) (r: reply): Prop :=
+    Inductive at_external: state -> query li1 -> Prop :=
+      | at_external_intro i s q:
+          Smallstep.at_external (L i) s q ->
+          at_external (existT _ i s) q.
+
+    Inductive after_external: state -> reply li1 -> state -> Prop :=
+      | after_external_intro i s r s':
+          Smallstep.after_external (L i) s r s' ->
+          after_external (existT _ i s) r (existT _ i s').
+
+    Definition final_state (s: state) (r: reply li2): Prop :=
       let (i, si) := s in Smallstep.final_state (L i) si r.
 
     Definition semantics :=
@@ -100,6 +52,8 @@ Module FComp.
         Smallstep.state := state;
         Smallstep.step := step;
         Smallstep.initial_state := initial_state;
+        Smallstep.at_external := at_external;
+        Smallstep.after_external := after_external;
         Smallstep.final_state := final_state;
         Smallstep.globalenv := fun i => Smallstep.globalenv (L i);
         Smallstep.symbolenv := ge;
@@ -107,14 +61,84 @@ Module FComp.
     End FLATCOMP.
 End FComp.
 
+(** * Resolution operator *)
+
+(** To go from the flat composition to horizontal composition, we
+  introduce the following resolution operator. [Res] eliminates
+  external calls to internal functions by replacing them with a nested
+  execution of the transition system. Each [Res.state] is a stack of
+  states of [L]: normal execution operates on the topmost state;
+  a recursive call into [L] pushes the nested initial state on the
+  stack; reaching a final state causes the topmost state to be popped
+  and the caller to be resumed, or returns to the environment when
+  we reach the last one. *)
+
+Module Res.
+  Section RESOLVE.
+    Context {li} (L: Smallstep.semantics li li).
+    Context (internal: query li -> bool).
+
+    Definition state := list (Smallstep.state L).
+
+    Inductive initial_state (q: query li): state -> Prop :=
+      | initial_state_intro s:
+          Smallstep.initial_state L q s ->
+          initial_state q (s :: nil).
+
+    Inductive at_external: state -> query li -> Prop :=
+      | at_external_intro s stk q':
+          Smallstep.at_external L s q' ->
+          internal q' = false ->
+          at_external (s :: stk) q'.
+
+    Inductive after_external: state -> reply li -> state -> Prop :=
+      | after_external_intro s stk r' s':
+          Smallstep.after_external L s r' s' ->
+          after_external (s :: stk) r' (s' :: stk).
+
+    Inductive final_state: state -> reply li -> Prop :=
+      | final_state_intro s r:
+          Smallstep.final_state L s r ->
+          final_state (s :: nil) r.
+
+    Inductive step ge : state -> trace -> state -> Prop :=
+      | step_internal s t s' stk:
+          Smallstep.step L ge s t s' ->
+          step ge (s :: stk) t (s' :: stk)
+      | step_call s stk qi si:
+          internal qi = true ->
+          Smallstep.at_external L s qi ->
+          Smallstep.initial_state L qi si ->
+          step ge (s :: stk) E0 (si :: s :: stk)
+      | step_return si ri s s' stk:
+          Smallstep.final_state L si ri ->
+          Smallstep.after_external L s ri s' ->
+          step ge (si :: s :: stk) E0 (s' :: stk).
+
+    Definition semantics: Smallstep.semantics li li :=
+      {|
+        Smallstep.state := state;
+        Smallstep.step := step;
+        Smallstep.initial_state := initial_state;
+        Smallstep.at_external := at_external;
+        Smallstep.after_external := after_external;
+        Smallstep.final_state := final_state;
+        Smallstep.globalenv := globalenv L;
+        Smallstep.symbolenv := symbolenv L;
+      |}.
+  End RESOLVE.
+End Res.
 
 (** * Horizontal composition *)
+
+(** Applying the resolution operator to the flat composition of
+  some transitions systems gives us horizontal composition. *)
 
 Module HComp.
   Section HCOMP.
     Context (ge: Senv.t).
-    Context {I} (L: I -> semantics).
-    Context (internal: query -> bool).
+    Context {li I} (L: I -> semantics li li).
+    Context (internal: query li -> bool).
 
     Definition semantics :=
       Res.semantics (FComp.semantics ge L) internal.
